execution/tests/FA2Tests/FA2TokenTests.v
@@ -1,0 +1,238 @@
+From ConCert Require Import Blockchain LocalBlockchain FA2Token FA2Interface.
+From ConCert Require Import Serializable.
+From ConCert Require Import LocalBlockchainTests.
+(* From Coq Require Import Morphisms. *)
+From ConCert Require Import Extras.
+From ConCert Require Import Containers.
+From ConCert Require Import BoundedN.
+Global Set Warnings "-extraction-logical-axiom".
+Require Import ZArith Strings.String.
+
+From QuickChick Require Import QuickChick. Import QcNotation.
+From ExtLib.Structures Require Import Functor Applicative.
+From ConCert.Execution.QCTests Require Import 
+	ChainGens TestUtils ChainPrinters SerializablePrinters TraceGens FA2Printers TestContracts.
+From RecordUpdate Require Import RecordUpdate.
+From Coq Require Import List.
+Import ListNotations.
+Import RecordSetNotations.
+(* For monad notations *)
+From ExtLib.Structures Require Import Monads.
+Import MonadNotation. Open Scope monad_scope.
+Close Scope address_scope.
+(* Notation "f 'o' g" := (compose f g) (at level 50). *)
+
+Definition LocalChainBase : ChainBase := ChainGens.LocalChainBase.
+
+(* Section Printers. *)
+Local Open Scope string_scope.
+
+Instance showFA2ClientMsg : Show FA2ClientMsg :=
+{|
+	show m := match m with
+            | Call_fa2_is_operator param => "Call_fa2_is_operator " ++ show param 
+            | Call_fa2_balance_of_param param => "Call_fa2_balance_of_param " ++ show param 
+            | Call_fa2_total_supply_param param => "Call_fa2_total_supply_param param " ++ show param
+            | Call_fa2_metadata_callback param => "Call_fa2_metadata_callback param " ++ show param
+            | Call_fa2_permissions_descriptor param => "Call_fa2_permissions_descriptor param " ++ show param
+						end
+|}.
+
+Instance showFA2ClientContractMsg : Show ClientMsg :=
+{|
+	show m := show m
+|}.
+
+Instance showFA2ClientState : Show ClientState :=
+{|
+  show t := "FA2ClientState{" 
+            ++ "fa2_caddr: " ++ show t.(fa2_caddr) ++ sep 
+            ++ "bit: " ++ show t.(bit) 
+            ++ "}"
+|}.
+
+Instance showFA2Setup : Show ClientSetup :=
+{|
+  show t := "FA2ClientSetup{" 
+            ++ "fa2_caddr_: " ++ show t.(fa2_caddr_) 
+            ++ "}"
+|}.
+
+Instance showFA2TransferHookMsg : Show FA2TransferHookMsg :=
+{|
+	show m := match m with
+            | set_permission_policy param => "set_permission_policy " ++ show param 
+						end
+|}.
+
+Instance showFA2TransferHookContractState : Show HookState :=
+{|
+  show t := "FA2TransferHookState{" 
+            ++ "fa2_caddr: " ++ show t.(hook_fa2_caddr) ++ sep 
+            ++ "policy: " ++ show t.(policy) ++ sep 
+            ++ "owner: " ++ show t.(owner) 
+            ++ "}"
+|}.
+
+Instance showFA2TransferHookContractSetup : Show HookSetup :=
+{|
+  show t := "FA2TransferHookSetup{" 
+            ++ "fa2_caddr_: " ++ show t.(hook_fa2_caddr_) ++ sep 
+            ++ "policy_: " ++ show t.(policy_) ++ sep 
+            ++ "}"
+|}.
+
+Close Scope string_scope.
+(* End Printers. *)
+
+
+(** example policies *)
+
+(* the policy which allows only token owners to transfer their own tokens. *)
+Definition policy_self_only : permissions_descriptor := {|
+  descr_self := self_transfer_permitted;
+  descr_operator := operator_transfer_denied;
+  descr_sender := owner_no_op;
+  descr_receiver := owner_no_op;
+  descr_custom := None;
+|}.
+
+(* the policy which allows only operators to transfer tokens. *)
+Definition policy_operators_only : permissions_descriptor := {|
+  descr_self := self_transfer_denied;
+  descr_operator := operator_transfer_permitted;
+  descr_sender := owner_no_op;
+  descr_receiver := owner_no_op;
+  descr_custom := None;
+|}.
+
+(* non-transferable token (neither token owner, nor operators can transfer tokens. *)
+Definition policy_no_transfers : permissions_descriptor := {|
+  descr_self := self_transfer_denied;
+  descr_operator := operator_transfer_denied;
+  descr_sender := owner_no_op;
+  descr_receiver := owner_no_op;
+  descr_custom := None;
+|}.
+
+(* the policy which allows both owners and operators to transfer tokens. *)
+Definition policy_all : permissions_descriptor := {|
+  descr_self := self_transfer_permitted;
+  descr_operator := operator_transfer_permitted;
+  descr_sender := owner_no_op;
+  descr_receiver := owner_no_op;
+  descr_custom := None;
+|}.
+
+Definition token_metadata_0 : token_metadata := {|
+  metadata_token_id := 0%N;
+  metadata_decimals := 8%N;
+|}.
+
+Definition token_setup : FA2Token.Setup := {|
+  setup_total_supply := [];
+  setup_tokens := FMap.add 0%N token_metadata_0 FMap.empty; 
+  initial_permission_policy := policy_all;
+|}.
+Definition deploy_fa2token : @ActionBody Base := create_deployment 0 FA2Token.contract token_setup.
+Definition token_contract_base_addr : Address := BoundedN.of_Z_const AddrSize 128%Z.
+
+Definition token_client_setup := build_clientsetup token_contract_base_addr.
+Definition deploy_fa2token_client : @ActionBody Base := create_deployment 0 client_contract token_client_setup.
+Definition client_contract_addr : Address := BoundedN.of_Z_const AddrSize 129%Z.
+
+Definition fa2hook_setup : HookSetup := {|
+  hook_fa2_caddr_ := token_contract_base_addr;
+  policy_ := policy_self_only; 
+|}.
+Definition deploy_fa2hook := create_deployment 0 hook_contract fa2hook_setup.
+Definition fa2hook_contract_addr : Address := BoundedN.of_Z_const AddrSize 130%Z.
+
+Definition chain_with_token_deployed : LocalChain :=  
+  unpack_option (my_add_block lc_initial 
+  [
+    build_act creator (act_transfer person_1 10);
+    build_act creator (act_transfer person_2 10);
+    build_act creator (act_transfer person_3 10);
+    build_act creator deploy_fa2token;
+    build_act creator deploy_fa2token_client;
+    build_act creator deploy_fa2hook
+  ]).
+
+Definition client_other_msg := @other_msg _ FA2ClientMsg _.
+
+Definition call_client_is_op_act :=
+  let params := Build_is_operator_param 
+      (Build_operator_param zero_address zero_address all_tokens)
+      (Build_callback is_operator_response None) in 
+  let msg := client_other_msg (Call_fa2_is_operator params) in
+  act_call client_contract_addr 0%Z (serialize ClientMsg _ msg).
+
+Definition chain1 : LocalChain :=
+  unpack_option (my_add_block chain_with_token_deployed 
+  [
+    build_act person_1 call_client_is_op_act
+  ]).
+
+Definition client_state lc := 
+  match (FMap.find client_contract_addr lc.(lc_contract_state)) with
+  | Some state => deserialize ClientState _ state
+  | None => None
+  end.
+Definition token_state lc := 
+  match (FMap.find token_contract_base_addr lc.(lc_contract_state)) with
+  | Some state => deserialize FA2Token.State _ state
+  | None => None
+  end.
+Compute (client_state chain1).
+(* Compute (show (token_state chain1)). *)
+
+Definition gClientMsg : G ClientMsg := 
+  let params := Build_is_operator_param 
+    (Build_operator_param zero_address zero_address all_tokens)
+    (Build_callback is_operator_response None) in
+  returnGen (client_other_msg (Call_fa2_is_operator params)).
+
+Definition gClientMsg' := 
+  (* let params := all_tokens in *)
+    (* (Build_operator_param zero_address zero_address all_tokens) in *)
+    (* (Build_callback is_operator_response None) in *)
+  returnGen all_tokens.
+
+Sample gClientMsg'.
+Sample (
+  msg <- gClientMsg' ;;
+  returnGen msg
+).
+
+Definition gClientAction := liftM (fun msg => 
+  Some (
+    build_act person_1 (
+      act_call token_contract_base_addr 0%Z (serialize ClientMsg _ msg)
+    )
+  )) gClientMsg.
+
+Definition gFA2ChainTraceList max_acts_per_block lc length := 
+  gLocalChainTraceList_fix lc (fun _ _=> 
+    gClientAction) length max_acts_per_block.
+
+Definition token_reachableFrom (lc : LocalChain) pf : Checker := 
+  @reachableFrom AddrSize lc (gFA2ChainTraceList 1) pf.
+
+Definition token_reachableFrom_implies_reachable (lc : LocalChain) pf1 pf2 : Checker := 
+  reachableFrom_implies_reachable lc (gFA2ChainTraceList 1) pf1 pf2.
+
+Sample gClientMsg.
+Sample (
+        msg <- gClientMsg;;
+        returnGen msg
+        ).
+Sample gClientAction.
+
+Sample (gFA2ChainTraceList 1 chain_with_token_deployed 4).
+
+
+
+
+
+
