execution/tests/FA2Tests/TestContracts.v
@@ -1,0 +1,253 @@
+From ConCert Require Import Blockchain LocalBlockchain FA2Token FA2Interface.
+From ConCert Require Import Serializable.
+From Coq Require Import Morphisms.
+
+Require Import Monads.
+Require Import Extras.
+Require Import Containers.
+Require Import Automation.
+From RecordUpdate Require Import RecordUpdate.
+From Coq Require Import List.
+Require Import ZArith.
+Import ListNotations.
+Import RecordSetNotations.
+
+Section FA2Client.
+Context {BaseTypes : ChainBase}.
+Set Primitive Projections.
+Set Nonrecursive Elimination Schemes.
+Open Scope N_scope.
+
+Inductive FA2ClientMsg :=
+  | Call_fa2_is_operator : is_operator_param -> FA2ClientMsg 
+  | Call_fa2_balance_of_param : list balance_of_response -> FA2ClientMsg
+  | Call_fa2_total_supply_param : list total_supply_response -> FA2ClientMsg
+  | Call_fa2_metadata_callback : list token_metadata -> FA2ClientMsg
+  | Call_fa2_permissions_descriptor : permissions_descriptor -> FA2ClientMsg.
+
+Global Instance FA2ClientMsg_serializable : Serializable FA2ClientMsg :=
+  Derive Serializable FA2ClientMsg_rect <
+    Call_fa2_is_operator, 
+    Call_fa2_balance_of_param, 
+    Call_fa2_total_supply_param,
+    Call_fa2_metadata_callback,
+    Call_fa2_permissions_descriptor>.
+
+Definition ClientMsg := @FA2ReceiverMsg BaseTypes FA2ClientMsg _.
+
+Record ClientState := 
+  build_clientstate {
+  fa2_caddr : Address;
+  bit : N;
+}.
+
+Record ClientSetup := 
+  build_clientsetup {
+  fa2_caddr_ : Address
+}.
+
+Instance state_settable : Settable _ :=
+  settable! build_clientstate <fa2_caddr; bit>.
+Instance setup_settable : Settable _ :=
+  settable! build_clientsetup <fa2_caddr_>.
+
+Section Serialization.
+
+Global Instance setup_serializable : Serializable ClientSetup :=
+  Derive Serializable ClientSetup_rect <build_clientsetup>.
+
+Global Instance state_serializable : Serializable ClientState :=
+	Derive Serializable ClientState_rect <build_clientstate>.
+
+Global Instance ClientMsg_serializable : Serializable ClientMsg := FA2Token.FA2ReceiverMsg_serializable.
+
+End Serialization.
+  
+Definition client_init (chain : Chain)
+								(ctx : ContractCallContext)
+								(setup : ClientSetup) : option ClientState := 
+  Some {|
+    fa2_caddr := setup.(fa2_caddr_);
+    bit := 0;
+	|}.
+
+Definition client_receive (chain : Chain)
+						 			 (ctx : ContractCallContext)
+									 (state : ClientState)
+									 (maybe_msg : option ClientMsg)
+									 : option (ClientState * list ActionBody) :=
+	match maybe_msg with
+  | Some (receive_is_operator is_op_response) => Some (state<| bit:= 42|>, [])
+  | Some (other_msg (Call_fa2_is_operator is_op_param)) => 
+      Some (state<| bit := 2|>, [act_call state.(fa2_caddr) 0%Z (@serialize FA2Token.Msg _ (FA2Token.msg_is_operator is_op_param))])
+  | _ => None 
+	end.
+
+Ltac solve_contract_proper :=
+  repeat
+    match goal with
+    | [|- ?x _  = ?x _] => unfold x
+    | [|- ?x _ _ = ?x _ _] => unfold x
+    | [|- ?x _ _ _ = ?x _ _ _] => unfold x
+    | [|- ?x _ _ _ _ = ?x _ _ _ _] => unfold x
+    | [|- ?x _ _ _ _ = ?x _ _ _ _] => unfold x
+    | [|- ?x _ _ _ _ _ = ?x _ _ _ _ _] => unfold x
+    | [|- Some _ = Some _] => f_equal
+    | [|- pair _ _ = pair _ _] => f_equal
+    | [|- (if ?x then _ else _) = (if ?x then _ else _)] => destruct x
+    | [|- match ?x with | _ => _ end = match ?x with | _ => _ end ] => destruct x
+    | [H: ChainEquiv _ _ |- _] => rewrite H in *
+    | _ => subst; auto
+    end.
+
+Lemma client_init_proper :
+  Proper (ChainEquiv ==> eq ==> eq ==> eq) client_init.
+Proof. repeat intro; solve_contract_proper.	Qed.
+
+Lemma client_receive_proper :
+  Proper (ChainEquiv ==> eq ==> eq ==> eq ==> eq) client_receive.
+Proof. repeat intro; solve_contract_proper. Qed.
+
+Definition client_contract : Contract FA2Client.ClientSetup ClientMsg FA2Client.ClientState :=
+  build_contract client_init client_init_proper client_receive client_receive_proper.
+
+End FA2Client.
+
+(* A contract which implements the transfer hook endpoint of FA2 *)
+(* Behavior is driven by a permission policy *)
+
+Section FA2TransferHook.
+Context {BaseTypes : ChainBase}.
+Set Primitive Projections.
+Set Nonrecursive Elimination Schemes.
+Open Scope N_scope.
+
+Inductive FA2TransferHookMsg :=
+  | set_permission_policy : permissions_descriptor -> FA2TransferHookMsg.
+
+Global Instance FA2TransferHookMsg_serializable : Serializable FA2TransferHookMsg :=
+  Derive Serializable FA2TransferHookMsg_rect <
+    set_permission_policy>.
+
+Definition TransferHookMsg := @FA2TransferHook BaseTypes FA2TransferHookMsg _.
+
+Record HookState := 
+  build_hookstate {
+    owner : Address;
+    hook_fa2_caddr : Address;
+    policy : permissions_descriptor;
+}.
+
+Record HookSetup := 
+  build_hooksetup {
+    hook_fa2_caddr_ : Address;
+    policy_ : permissions_descriptor;
+}.
+
+Instance hookstate_settable : Settable _ :=
+  settable! build_hookstate <owner; hook_fa2_caddr; policy>.
+Instance hooksetup_settable : Settable _ :=
+  settable! build_hooksetup <hook_fa2_caddr_; policy_>.
+
+Section Serialization.
+
+Global Instance hooksetup_serializable : Serializable HookSetup :=
+  Derive Serializable HookSetup_rect <build_hooksetup>.
+
+Global Instance hookstate_serializable : Serializable HookState :=
+	Derive Serializable HookState_rect <build_hookstate>.
+
+End Serialization.
+  
+Definition hook_init (chain : Chain)
+								(ctx : ContractCallContext)
+								(setup : HookSetup) : option HookState := 
+  Some {|
+    owner := ctx.(ctx_from);
+    hook_fa2_caddr := setup.(hook_fa2_caddr_);
+    policy := setup.(policy_);
+	|}.
+
+Definition returnIf (cond : bool) := if cond then None else Some tt.
+
+Definition check_transfer_permissions (tr : transfer_descriptor)
+                                      (operator : Address)
+                                      (state : HookState) 
+                                      : option unit :=
+  if (address_eqb tr.(transfer_descr_from_) operator)
+  then if (FA2Token.policy_disallows_self_transfer state.(policy))
+    then None 
+    else Some tt
+  else if (FA2Token.policy_disallows_operator_transfer state.(policy))
+    then None
+    else Some tt.
+
+(* called whenever this hook receives a transfer from the FA2 contract *)
+(* checks the permission policy, and if all transfers are valid, 
+   forwards the transfers to the 'msg_receive_hook_transfer' endpoint of the FA2 Contract *)
+Definition on_hook_receive_transfer (caller : Address)
+                                    (param : transfer_descriptor_param)
+                                    (state : HookState)
+                                    : option (list ActionBody) :=
+  do _ <- returnIf (negb (address_eqb caller state.(hook_fa2_caddr))) ;
+  do _ <- returnIf (negb (address_eqb param.(transfer_descr_fa2) state.(hook_fa2_caddr))) ;
+  let operator := param.(transfer_descr_operator) in
+  let check_transfer_iterator tr acc :=
+    do _ <- check_transfer_permissions tr operator state ;
+    Some tt in
+  (* check if all transfers satisfy the permission policy. If at least one does not, the whole operation fails *)
+  do _ <- fold_right check_transfer_iterator (Some tt) param.(transfer_descr_batch) ;
+  (* send out transfer action *)
+  let msg := @serialize FA2Token.Msg _ (msg_receive_hook_transfer param) in
+  Some [(act_call caller 0%Z msg)].
+
+Definition try_update_permission_policy (caller : Address)
+                                    (new_policy : permissions_descriptor)
+                                    (state : HookState)
+                                    : (option HookState) :=
+  do _ <- returnIf (negb (address_eqb caller state.(owner))) ;
+  Some (state<| policy := new_policy |>).
+
+Definition hook_receive (chain : Chain)
+						 			 (ctx : ContractCallContext)
+									 (state : HookState)
+									 (maybe_msg : option TransferHookMsg)
+                   : option (HookState * list ActionBody) :=
+  let sender := ctx.(ctx_from) in
+  let without_actions := option_map (fun new_state => (new_state, [])) in
+	let without_statechange := option_map (fun acts => (state, acts)) in
+  match maybe_msg with
+  | Some (transfer_hook param) => without_statechange (on_hook_receive_transfer sender param state)
+  | Some (hook_other_msg (set_permission_policy policy)) => without_actions (try_update_permission_policy sender policy state)
+  | _ => None 
+	end.
+
+Ltac solve_contract_proper :=
+  repeat
+    match goal with
+    | [|- ?x _  = ?x _] => unfold x
+    | [|- ?x _ _ = ?x _ _] => unfold x
+    | [|- ?x _ _ _ = ?x _ _ _] => unfold x
+    | [|- ?x _ _ _ _ = ?x _ _ _ _] => unfold x
+    | [|- ?x _ _ _ _ = ?x _ _ _ _] => unfold x
+    | [|- ?x _ _ _ _ _ = ?x _ _ _ _ _] => unfold x
+    | [|- Some _ = Some _] => f_equal
+    | [|- pair _ _ = pair _ _] => f_equal
+    | [|- (if ?x then _ else _) = (if ?x then _ else _)] => destruct x
+    | [|- match ?x with | _ => _ end = match ?x with | _ => _ end ] => destruct x
+    | [H: ChainEquiv _ _ |- _] => rewrite H in *
+    | _ => subst; auto
+    end.
+
+Lemma hook_init_proper :
+  Proper (ChainEquiv ==> eq ==> eq ==> eq) hook_init.
+Proof. repeat intro; solve_contract_proper.	Qed.
+
+Lemma hook_receive_proper :
+  Proper (ChainEquiv ==> eq ==> eq ==> eq ==> eq) hook_receive.
+Proof. repeat intro; solve_contract_proper. Qed.
+
+Definition hook_contract : Contract HookSetup TransferHookMsg HookState :=
+  build_contract hook_init hook_init_proper hook_receive hook_receive_proper.
+
+End FA2TransferHook.
