execution/tests/Playground.v
@@ -1,19 +1,38 @@
-From ConCert Require Import Serializable.
-(* Remove Hints BoundedN_equivalence. *)
-Set Typeclasses Debug Verbosity 1.
-(* Existing Instance ser_value_equivalence | 0. *)
-(* Check deserialize. *)
-(* Print All Dependencies Serializable. *)
-(* Transparent deserialize. *)
+(* From ConCert Require Import Blockchain LocalBlockchain FA2Token FA2Interface. *)
+(* From ConCert Require Import Serializable.
+From ConCert Require Import LocalBlockchainTests.
+(* From Coq Require Import Morphisms. *)
+From ConCert Require Import Extras.
+From ConCert Require Import Containers.
+From ConCert Require Import BoundedN.
+Global Set Warnings "-extraction-logical-axiom".
+Require Import ZArith Strings.String.
 
+From QuickChick Require Import QuickChick. Import QcNotation.
+From ExtLib.Structures Require Import Functor Applicative.
+From ConCert.Execution.QCTests Require Import 
+	ChainGens TestUtils ChainPrinters SerializablePrinters TraceGens FA2Printers TestContracts.
+From RecordUpdate Require Import RecordUpdate.
+From Coq Require Import List.
+Import ListNotations.
+Import RecordSetNotations.
+(* For monad notations *)
+From ExtLib.Structures Require Import Monads.
+Import MonadNotation. Open Scope monad_scope.
+Close Scope address_scope. *)
+From QuickChick Require Import QuickChick. Import QcNotation.
+From ExtLib.Structures Require Import Functor Applicative.
+Import MonadNotation. 
+(* Open Scope monad_scope. *)
 
-Check deserialize.
-Typeclasses eauto := debug.
+(* From ConCert.Execution.QCTests Require Import 
+	ChainGens TestUtils ChainPrinters SerializablePrinters TraceGens FA2Printers TestContracts. *)
 
-Example ex2 : SerializedValue := serialize 2.
-Existing Instance nat_serializable | 0.
-Existing Instance bool_serializable | 0.
-Example ex3 := deserialize ex2.
-Compute ex3.
-Compute (deserialize ex2).
-Check (deserialize ex2).
+Definition a : G nat := 
+  returnGen 1.
+
+Definition b : G nat := 
+	v <- a ;;
+	returnGen v.
+	
+Sample b.
